Refine_Imperative_HOL/IICF/Intf/IICF_Set.thy
@@ -4,13 +4,88 @@ imports "../../Sepref"
 begin
 
 subsection \<open>Operations\<close>
+
+(*
 definition [simp]: "op_set_is_empty s \<equiv> s={}"
 lemma op_set_is_empty_param[param]: "(op_set_is_empty,op_set_is_empty)\<in>\<langle>A\<rangle>set_rel \<rightarrow> bool_rel" by auto
+*)
+
 
 context 
   notes [simp] = IS_LEFT_UNIQUE_def (* Argh, the set parametricity lemmas use single_valued (K\<inverse>) here. *)
 begin
 
+
+context
+  fixes t ::  "nat"
+begin
+  definition "mop_set_empty = SPECT [ {} \<mapsto> enat t ]"
+
+  lemma mop_set_empty: "tt \<le> TTT Q (SPECT [ {} \<mapsto> t ]) \<Longrightarrow> tt
+           \<le> TTT Q (mop_set_empty)" unfolding mop_set_empty_def by simp
+
+  sepref_register "mop_set_empty" 
+  print_theorems 
+end
+
+
+context
+  fixes t ::  "'c set \<Rightarrow> nat"
+begin
+  definition "mop_set_pick S = SPECT (emb (\<lambda>x. x\<in>S) (t S))"
+
+  lemma  mop_set_pick: "tt \<le> TTT Q (SPECT (emb (\<lambda>x. x\<in>S) (t S))) 
+        \<Longrightarrow> tt \<le> TTT Q (mop_set_pick S)" unfolding mop_set_pick_def by simp
+
+  lemma progress_mop_set_pick[progress_rules]: "t S > 0 \<Longrightarrow> progress (mop_set_pick S)"
+    unfolding mop_set_pick_def by (auto intro: progress_rules simp add:   zero_enat_def) 
+
+  sepref_register "mop_set_pick" 
+  print_theorems 
+end
+
+
+context
+  fixes t:: "'a set \<Rightarrow> nat" 
+begin
+  definition "mop_set_member x S = SPECT [ x \<in> S \<mapsto> enat (t S) ]"
+  sepref_register "mop_set_member" 
+  print_theorems 
+end
+
+ 
+
+context
+  fixes t ::  "'c set \<Rightarrow> nat"
+begin
+  definition "mop_set_del S x = SPECT [ S - {x} \<mapsto> (t S)]"
+
+  lemma  mop_set_del: "tt \<le> TTT Q (SPECT [ S - {x} \<mapsto> (t S)]) 
+        \<Longrightarrow> tt \<le> TTT Q (mop_set_del S x)" unfolding mop_set_del_def by simp
+
+
+  lemma progress_mop_set_del[progress_rules]: "t S > 0 \<Longrightarrow> progress (mop_set_del S x)"
+      unfolding mop_set_del_def  by (auto intro: progress_rules simp add:   zero_enat_def) 
+
+  sepref_register "mop_set_del" 
+  print_theorems 
+end
+
+
+context 
+  fixes t :: "'c set \<Rightarrow> nat"
+begin
+
+  definition "mop_set_insert x S = SPECT [insert x S \<mapsto> t S]"
+
+  lemma mop_set_insert: "tt \<le> TTT Q (SPECT [ (insert x S) \<mapsto> t S]) \<Longrightarrow>
+         tt \<le> TTT Q (mop_set_insert x S)" unfolding mop_set_insert_def by simp
+
+  sepref_register "mop_set_insert" 
+  print_theorems 
+end
+
+(*
 sepref_decl_op set_empty: "{}" :: "\<langle>A\<rangle>set_rel" .
 sepref_decl_op (no_def) set_is_empty: op_set_is_empty :: "\<langle>A\<rangle>set_rel \<rightarrow> bool_rel" .
 sepref_decl_op set_member: "(\<in>)" :: "A \<rightarrow> \<langle>A\<rangle>set_rel \<rightarrow> bool_rel" where "IS_LEFT_UNIQUE A" "IS_RIGHT_UNIQUE A" .
@@ -26,12 +101,16 @@ sepref_decl_op set_subset: "(\<subset>)" :: "\<langle>A\<rangle>set_rel \<righta
 (* TODO: We may want different operations here: pick with predicate returning option,
   pick with remove, ... *)    
 sepref_decl_op set_pick: "REST" :: "[\<lambda>s. s\<noteq>{}]\<^sub>f \<langle>K\<rangle>set_rel \<rightarrow> K" by auto
+*)
+
 
 end
 
 (* TODO: Set-pick. Move from where it is already defined! *)
 
 subsection \<open>Patterns\<close>
+
+(*
 lemma pat_set[def_pat_rules]:
   "{} \<equiv> op_set_empty"
   "(\<in>) \<equiv> op_set_member"    
@@ -51,8 +130,9 @@ lemma pat_set2[pat_rules]:
   "SPEC$(\<lambda>\<^sub>2x. (\<in>) $x$s) \<equiv> op_set_pick s"
   "RES$s \<equiv> op_set_pick s"
   by (auto intro!: eq_reflection)
+*)
 
-
+(*
 locale set_custom_empty = 
   fixes empty and op_custom_empty :: "'a set"
   assumes op_custom_empty_def: "op_custom_empty = op_set_empty"
@@ -65,6 +145,8 @@ begin
     "mop_set_empty = RETURN op_custom_empty"
     unfolding op_custom_empty_def by simp_all
 end
+*)
+
 
 end
 
