Examples/Fib.thy
@@ -1,6 +1,5 @@
 theory Fib  
   imports "../Refine_Imperative_HOL/Sepref" "SepLogicTime_RBTreeBasic.RBTree_Impl"
-    "../Set_Impl2" 
 begin
 
 
