RefineMonadicVCG.thy
@@ -358,74 +358,14 @@ thm T_pw refine_pw_simps
 thm pw_le_iff
 
 
+subsection "progress solver"
 
-subsection \<open>Progress rules and solver\<close>
-
-named_theorems progress_rules
-
-lemma progress_SELECT_iff: "progress (SELECT P T) \<longleftrightarrow> T > 0"
-  unfolding progress_def SELECT_def emb'_def by (auto split: option.splits)
-
-lemmas [progress_rules] = progress_SELECT_iff[THEN iffD2]
-
-lemma progress_REST_iff: "progress (REST [x \<mapsto> t]) \<longleftrightarrow> t>0"
-  by (auto simp: progress_def)
-
-lemmas [progress_rules] = progress_REST_iff[THEN iffD2]
-
-lemma progress_ASSERT_bind[progress_rules]: "\<lbrakk>\<Phi> \<Longrightarrow> progress (f ()) \<rbrakk> \<Longrightarrow> progress (ASSERT \<Phi>\<bind>f)"
-  apply (cases \<Phi>)
-  apply (auto simp: progress_def)
-  done
-
-
-lemma progress_SPECT_emb[progress_rules]: "t > 0 \<Longrightarrow> progress (SPECT (emb P t))" by(auto simp: progress_def emb'_def)
-
-
-lemma Sup_Some: "Sup (S::enat option set) = Some e \<Longrightarrow> \<exists>x\<in>S. (\<exists>i. x = Some i)"
-  unfolding Sup_option_def by (auto split: if_splits)
-
-lemma progress_bind[progress_rules]: assumes "progress m \<or> (\<forall>x. progress (f x))"
-  shows "progress (m\<bind>f)"
-proof  (cases m)
-  case FAILi
-  then show ?thesis by (auto simp: progress_def)
-next
-  case (REST x2)   
-  then show ?thesis unfolding  bindT_def progress_def apply safe
-  proof (goal_cases)
-    case (1 s' M y)
-    let ?P = "\<lambda>fa. \<exists>x. f x \<noteq> FAILT \<and>
-             (\<exists>t1. \<forall>x2a. f x = SPECT x2a \<longrightarrow> fa = map_option ((+) t1) \<circ> x2a \<and> x2 x = Some t1)"
-    from 1 have A: "Sup {fa s' |fa. ?P fa} = Some y" apply simp
-      apply(drule nrest_Sup_SPECT_D[where x=s']) by (auto split: nrest.splits)
-    from Sup_Some[OF this] obtain fa i where P: "?P fa" and 3: "fa s' = Some i"   by blast 
-    then obtain   x t1 x2a  where  a3: "f x = SPECT x2a"
-      and "\<forall>x2a. f x = SPECT x2a \<longrightarrow> fa = map_option ((+) t1) \<circ> x2a" and a2: "x2 x = Some t1"  
-      by fastforce 
-    then have a1: " fa = map_option ((+) t1) \<circ> x2a" by auto
-    have "progress m \<Longrightarrow> t1 > 0" apply(drule progressD)
-      using 1(1) a2 a1 a3 by auto  
-    moreover
-    have "progress (f x) \<Longrightarrow> x2a s' > Some 0"  
-      using   a1 1(1) a2 3  by (auto dest!: progressD[OF _ a3])   
-    ultimately
-    have " t1 > 0 \<or> x2a s' > Some 0" using assms by auto
-
-    then have "Some 0 < fa s'" using   a1  3 by auto
-    also have "\<dots> \<le> Sup {fa s'|fa. ?P fa}" 
-      apply(rule Sup_upper) using P by blast
-    also have "\<dots> = M s'" using A 1(3) by simp
-    finally show ?case .
-  qed 
-qed
 
 
 method progress methods solver = 
   (rule asm_rl[of "progress _"] , (simp split: prod.splits | intro allI impI conjI | determ \<open>rule progress_rules\<close> | rule disjI1; progress \<open>solver\<close>; fail | rule disjI2; progress \<open>solver\<close>; fail | solver)+) []
 method progress' methods solver = 
   (rule asm_rl[of "progress _"] , (vcg_split_case | intro allI impI conjI | determ \<open>rule progress_rules\<close> | rule disjI1 disjI2; progress'\<open>solver\<close> | (solver;fail))+) []
-
 
 
 subsection \<open>WHILET refine\<close>
